Transport-based fibrancy. Prove U is fibrant, Bool is fibrant.

theories/translation_fib.v
@@ -88,82 +88,41 @@ Definition ytEl_funct@{i j} {p q} {f : yt@{i} p} (α : q ≤ p) :
   ytEl@{i j} f -> ytEl@{i j} (yt_funct@{i} α f) :=
 fun s => mkYtEl@{i j} q (yt_funct α f) (α ⋅ s.(ytel0)) (α ⋅ s.(ytel1)).
 
-(* generating cofibrations, AFH style *)
-(* question : do we want to make it into a presheaf to
-   get functoriality ?  *)
-
-Definition cofib (p : ℙ) : Set.
-Admitted.
-
-Definition cofib_funct {p q : ℙ} (α : q ≤ p) :
-  cofib p -> cofib q.
-Admitted.
-
-Definition cofibface {p q : ℙ} (b : cofib p) (α : q ≤ p) : bool.
-Admitted.
-
-Definition tubeface {p q : ℙ} (b : cofib p) (α : q ≤ S p) : bool.
-Admitted.
-
-(* sections of yoneda(S p) -> yoneda(p) *)
-
-Definition lid (p : ℙ) : Set.
-Admitted.
-
-Definition lidface {p : ℙ} (l : lid p) : p ≤ S p.
-Admitted.
-
-(* Partial sections of a presheaf over yoneda(p) *)
-
-Record partialEl@{i j} {p : ℙ} (t : yt@{i} p)
-  (domain : forall q (α : q ≤ p), bool) :=
-mkPartialEl {
-  pe_el : forall q (α : q ≤ p) (Hα : domain q α ≡ true),
-    ytEl@{i j} (yt_funct@{i} α t) ;
-  pe_compat : forall q (α : q ≤ p) (Hα : domain q α ≡ true)
-    r (β : r ≤ q) (Hβ : domain r (α ∘ β) ≡ true),
-    ytEl_funct β (pe_el q α Hα) ≡ pe_el r (α ∘ β) Hβ ;
-}.
-
-Arguments pe_el {_ _ _}.
-Arguments pe_compat {_ _ _}.
-
-Definition tubeEl@{i j} {p : ℙ} (t : yt@{i} (S p))
-  (b : cofib p)
- := partialEl t (fun q α => tubeface b α).
-
-Record lidEl@{i j} {p : ℙ} {t : yt@{i} (S p)}
-  {b : cofib p} (e : tubeEl@{i j} t b) (l : lid p) :=
-mkLidEl {
-  le_el : ytEl@{i j} (yt_funct@{i} (lidface l) t) ;
-  le_compat : forall q (α : q ≤ p)
-    (Hα : tubeface b ((lidface l) ∘ α) ≡ true),
-    exteq_ytEl (ytEl_funct α le_el) (e.(pe_el) q ((lidface l) ∘ α) Hα) ;
-}.
-
-(* With this, we can define a fibration structure *)
-(* A presheaf over yoneda(p) is fibrant if all partial sections
-   have fillers *)
-
+(* 
 Definition fibstruct@{i j} (p : ℙ)
   (t0 : forall q (α : q ≤ S p), Type@{i})
   (t1 : forall q (α : q ≤ S p) (s : forall r (β : r ≤ q), t0 r (α ∘ β)), SProp)
   : Type@{i} :=
-forall (b : cofib p) (e : tubeEl@{i j} (mkYT (S p) t0 t1) b)
-  (l : lid p) (le : lidEl@{i j} e l) (l' : lid p),
-  lidEl@{i j} e l'.
-
-(* Type of fibrant presheaves over yoneda(p) *)
+ytEl (mkYT p (side_0 ⋅ t0) (side_0 ⋅ t1)) -> ytEl (mkYT p (side_1 ⋅ t0) (side_1 ⋅ t1)).
+ *)
 
 Record yft@{i j} (p : ℙ) := mkYFT {
   yft0 : forall q (α : q ≤ p), Type@{i};
   yft1 : forall q (α : q ≤ p), (forall r (β : r ≤ q), yft0 r (α ∘ β)) -> SProp;
-  yftfib : forall q (α : S q ≤ p), fibstruct@{i j} q (α ⋅ yft0) (α ⋅ yft1);
+  yftfibl0 : forall q (α : S q ≤ p) 
+    (s0 : forall r (β : r ≤ q), yft0 r (α ∘ side_0 ∘ β)) 
+    (s1 : forall r (β : r ≤ q), yft1 r (α ∘ side_0 ∘ β) (fun r0 β0 => s0 r0 (β ∘ β0))),
+    yft0 q (α ∘ side_1) ;
+  yftfibl1 : forall q (α : S q ≤ p)
+    (s0 : forall r (β : r ≤ q), yft0 r (α ∘ side_0 ∘ β)) 
+    (s1 : forall r (β : r ≤ q), yft1 r (α ∘ side_0 ∘ β) (fun r0 β0 => s0 r0 (β ∘ β0))),
+    yft1 q (α ∘ side_1) (fun r (β : r ≤ q) => yftfibl0 r (α ∘ promote β) (β ⋅ s0) (β ⋅ s1)) ;
+  yftfibr0 : forall q (α : S q ≤ p) 
+    (s0 : forall r (β : r ≤ q), yft0 r (α ∘ side_1 ∘ β)) 
+    (s1 : forall r (β : r ≤ q), yft1 r (α ∘ side_1 ∘ β) (fun r0 β0 => s0 r0 (β ∘ β0))),
+    yft0 q (α ∘ side_0) ;
+  yftfibr1 : forall q (α : S q ≤ p)
+    (s0 : forall r (β : r ≤ q), yft0 r (α ∘ side_1 ∘ β)) 
+    (s1 : forall r (β : r ≤ q), yft1 r (α ∘ side_1 ∘ β) (fun r0 β0 => s0 r0 (β ∘ β0))),
+    yft1 q (α ∘ side_0) (fun r (β : r ≤ q) => yftfibr0 r (α ∘ promote β) (β ⋅ s0) (β ⋅ s1))
 }.
 
 Arguments yft0 {_}.
 Arguments yft1 {_}.
-Arguments yftfib {_}.
+Arguments yftfibl0 {_}.
+Arguments yftfibl1 {_}.
+Arguments yftfibr0 {_}.
+Arguments yftfibr1 {_}.
 
 Definition yft_funct@{i j} {p q : ℙ} (α : q ≤ p) :
   yft@{i j} p -> yft@{i j} q :=
@@ -171,7 +130,10 @@ fun f =>
 {|
   yft0 := α · yft0 f;
   yft1 := α ⋅ yft1 f;
-  yftfib := α ⋅ yftfib f;
+  yftfibl0 := α ⋅ yftfibl0 f;
+  yftfibl1 := α ⋅ yftfibl1 f;
+  yftfibr0 := α ⋅ yftfibr0 f;
+  yftfibr1 := α ⋅ yftfibr1 f;
 |}.
 
 (* original version had an extensional version of this *)
@@ -187,51 +149,6 @@ Proof.
 refine (fun x => _).
 refine (J_seq _ (α ⋅ A0) (fun a _ => (a r β).(yft0) r !) x _ (A1 q α)).
 Defined.
-
-(* Definition yftR@{i j k} {p : ℙ} (s : forall q : nat, q ≤ p -> yft@{i j} q) : SProp :=
-  forall q (α : q ≤ p),
-    seq@{k} ((s q α).(yft0) q !) ((s p !).(yft0) q α).
-
-Definition cast0 {p : ℙ}
-  (A0 : forall q (α : q ≤ p), yft q)
-  (A1 : forall q (α : q ≤ p), yftR (α · A0))
-  {q} (α : q ≤ p) {r} (β : r ≤ q) :
-  (A0 r (α ∘ β)).(yft0) r ! -> (A0 q α).(yft0) r β.
-Proof.
-refine (fun x => _).
-refine (J_seq _ _ (fun a _ => a) x _ (A1 q α r β)).
-Defined. *)
-
-(* Definition yftR@{i j k} {p : ℙ} (s : forall q : nat, q ≤ p -> yft@{i j} q) : SProp :=
-  seq@{k} s (fun q α => yft_funct@{i j} α (s p !)). *)
-
-(* Definition cast0 {p : ℙ}
-  (A0 : forall q (α : q ≤ p), yft q)
-  (A1 : forall q (α : q ≤ p), yftR (α · A0))
-  {q} (α : q ≤ p) {r} (β : r ≤ q) :
-  (A0 r (α ∘ β)).(yft0) r ! -> (A0 q α).(yft0) r β.
-Proof.
-refine (fun x => _).
-refine (J_seq _ (α ⋅ A0) (fun a _ => (a r β).(yft0) r !) x _ (A1 q α)).
-Defined. *)
-
-(* Definition seq_yftAlt {p : ℙ}
-  {t1 t2 : ytEl {| yt0 := fun q (_ : q ≤ p) => yft q ;
-                   yt1 := fun q (_ : q ≤ p) s => yftR s ; |}} :
-  t1.(ytel0) p ! ≡ t2.(ytel0) p ! -> t1 ≡ t2.
-Proof.
-intro H. apply seq_ytEl.
-pose proof (ytel1 t1 p !) as H1 ; simpl in H1.
-refine (J_seqs _ _
-  (fun x _ => x ≡ ytel0 t2) _ (ytel0 t1) (ssym H1)).
-refine (J_seqs _ (ytel0 t2 p !)
-  (fun x _ => (fun q α => yft_funct α x) ≡ ytel0 t2)
-  _ (ytel0 t1 p !) (ssym H)).
-pose proof (ytel1 t2 p !) as H2 ; simpl in H2.
-refine (J_seqs _ _
-  (fun x _ => (fun q α => yft_funct α (ytel0 t2 p !)) ≡ x)
-  (srefl _) (ytel0 t2) (ssym H2)).
-Defined. *)
 
 (* Sections of fibrant presheaves over yoneda(p) *)
 
@@ -257,115 +174,6 @@ Definition yftEl_funct@{i j k} {p q} {f : yft@{i j} p} (α : q ≤ p) :
   yftEl@{i j k} f -> yftEl@{i j k} (yft_funct@{i j} α f) :=
 fun s => mkYftEl@{i j k} q (yft_funct α f) (α ⋅ s.(yftel0)) (α ⋅ s.(yftel1)).
 
-(* Partial fibrant presheaves over yoneda(S p) *)
-
-Definition partialYft@{i j k l} {p : ℙ}
-  (domain : forall q (α : q ≤ p), bool) :=
-  partialEl@{k l}
-    {| yt0 := fun q (_ : q ≤ p) => yft@{i j} q ;
-       yt1 := fun q (_ : q ≤ p) s => yftR@{i j k} s ; |} domain.
-
-Definition tubeYft@{i j k l} {p : ℙ} (b : cofib p) :=
-  tubeEl@{k l}
-    {| yt0 := fun q (_ : q ≤ S p) => yft@{i j} q ;
-       yt1 := fun q (_ : q ≤ S p) s => yftR@{i j k} s ; |} b.
-
-Definition lidYft@{i j k l} {p : ℙ} {b : cofib p}
-  (t : tubeYft@{i j k l} b) (l : lid p) :=
-  lidEl@{k l} t l.
-
-(* Sections of a partial fibrant presheaf over yoneda(S p) *)
-(* this definition is function-based, and therefore not very
-   extensional. It is quite possible we will need to make it
-   list-based so that partial types satisfy some extensionality *)
-
-(* Definition boxYftEq {p : ℙ} {b : box p} (t : boxYft b)
-  {q : ℙ} (α : q ≤ S p) (Hα : boxface b α ≡ true)
-  {r : ℙ} (β : r ≤ q) (Hβ : boxface b (α ∘ β) ≡ true) :
-  ytel0 (be_el t r (α ∘ β) Hβ) r ! ≡ yft_funct β (ytel0 (be_el t q α Hα) q !).
-Proof.
-unshelve refine (J_seqs _ (ytEl_funct β (be_el t q α Hα))
-  (fun x _ => ytel0 x r ! ≡ yft_funct β (ytel0 (be_el t q α Hα) q !))
-  _ (be_el t r (α ∘ β) Hβ) (be_compat t _ α Hα _ β Hβ)).
-exact (ytel1 (be_el t q α Hα) q ! r β).
-Defined.
-
-Record boxYftEl {p : ℙ} {b : box p} (t : boxYft b) : Type :=
-mkBoxYftEl {
-  bye0 : forall q (α : q ≤ S p) (Hα : boxface b α ≡ true),
-    yftEl (ytel0 (t.(be_el) q α Hα) q !) ;
-  bye1 : forall q (α : q ≤ S p) (Hα : boxface b α ≡ true)
-    r (β : r ≤ q) (Hβ : boxface b (α ∘ β) ≡ true),
-    yftEl_funct β (bye0 q α Hα) ≡ transp_seq yftEl (bye0 r (α ∘ β) Hβ) (boxYftEq t α Hα β Hβ) ;
-}.
-
-Definition boxYftEl' {p : ℙ} {b : box p} (t : boxYft b) : Type.
-Proof.
-  unshelve refine ((match (boxface b !) as bl return (boxface b ! ≡ bl) -> Type with
-    | true => (fun Hα => _)
-    | false => (fun _ => _)
-    end) (srefl _)).
-  - exact (yftEl (ytel0 (t.(be_el) _ ! Hα) (S p) !)).
-  - exact (boxYftEl t).
-Defined. *)
-
-(* *)
-
-Definition tubeGlue@{i j k l} {p : ℙ}
-  {b : cofib p} (t : tubeYft@{i j k l} b)
-  {l : lid p} (lt : lidYft@{i j k l} t l)
-  (l' : lid p) {q} (α : q ≤ p) : Type@{i}.
-Proof.
-Admitted.
-
-Definition tubeGlue_funct@{i j k l} {p : ℙ}
-  {b : cofib p} {t : tubeYft@{i j k l} b}
-  {l : lid p} {lt : lidYft@{i j k l} t l}
-  {l' : lid p} {q} {α : q ≤ p}
-  {r} (β : r ≤ q) :
-  tubeGlue@{i j k l} t lt l' α -> tubeGlue@{i j k l} t lt l' (α ∘ β).
-Proof.
-Admitted.
-
-Definition tubeGlueR@{i j k l} {p : ℙ}
-  {b : cofib p} (t : tubeYft@{i j k l} b)
-  {l : lid p} (lt : lidYft@{i j k l} t l)
-  (l' : lid p) {q} (α : q ≤ p) :
-  (forall r (β : r ≤ q), tubeGlue t lt l' (α ∘ β)) -> SProp.
-Proof.
-refine (fun s => _).
-exact (forall r (β : r ≤ q), s r β ≡ tubeGlue_funct β (s q !)).
-Defined.
-
-Definition tubeGlueFib@{i j k l} {p : ℙ}
-  {b : cofib p} (t : tubeYft@{i j k l} b)
-  {l : lid p} (lt : lidYft@{i j k l} t l)
-  (l' : lid p) {q} (α : S q ≤ p) :
-  fibstruct q (fun _ β => tubeGlue t lt l' (α ∘ β))
-    (fun _ β => tubeGlueR t lt l' (α ∘ β)).
-Proof.
-Admitted.
-
-Definition tubeGlueLid@{i j k l} {p : ℙ}
-  {b : cofib p} (t : tubeYft@{i j k l} b)
-  {l : lid p} (lt : lidYft@{i j k l} t l)
-  (l' : lid p) :
-  lidYft@{i j k l} t l'.
-Proof.
-unshelve econstructor.
-- unfold yt_funct ; simpl. unshelve econstructor ; simpl.
-  + refine (fun q α => _).
-    unshelve econstructor.
-    * refine (if (tubeface b ((lidface l') ∘ α)) then _ else _).
-      admit.
-      admit. (* refine (fun r β => tubeGlue@{i j k l} t lt l' (α ∘ β)). *)
-    * admit. (*  refine (fun r β => tubeGlueR@{i j k l} t lt l' (α ∘ β)). *)
-    * admit. (* refine (fun r β => tubeGlueFib t lt l' (α ∘ β)). *)
-  + refine (fun q α => _). simpl.
-    admit.
-- unshelve refine (fun q α Hα r β => _) ; simpl.
-  reflexivity.
-Admitted.
 
 (* Universe of fibrant types *)
 
@@ -377,9 +185,10 @@ Proof.
 unshelve econstructor.
 - exact (fun q α => yft q).
 - refine (fun q α s => yftR s).
-- refine (fun q α b e l le l' => _).
-  change (tubeYft b) in e. change (lidYft e l) in le. change (lidYft e l').
-  refine (tubeGlueLid e le l').
+- refine (fun q α s0 s1 => s0 q !).
+- refine (fun q α s0 s1 => s0 q !).
+- refine (fun q α s0 s1 => s1 q !).
+- refine (fun q α s0 s1 => s1 q !).
 Defined.
 
 Definition U1 (p : ℙ) : psh1 Uᶠ p (fun q α => U0 q).
@@ -421,8 +230,6 @@ Proof.
   refine (fun q α => U1 q).
 Defined.
 
-
-
 (* From these definition, it is quite clear that
    * Type0 p : El0 p (Type0 p)
    * Type1 p : El1 p (Type0 p) (Type1 p) *)
@@ -434,16 +241,13 @@ fun s => s ≡ fun q α => s p !.
 
 Definition bool0 {p} : @El0 p Type0.
 Proof.
-unshelve refine (fun q α => mkYFT _ _ _ _).
-- unshelve refine (fun r β => bool).
-- unshelve refine (fun r β s => boolR s).
-- unshelve refine (fun r β b e l le l' => _).
-  unshelve econstructor.
-  + unfold yt_funct ; simpl.
-    unshelve econstructor ; simpl.
-    apply falso.
-    apply sfalso.
-  + apply sfalso.
+unshelve econstructor.
+- refine (fun r β => bool).
+- refine (fun r β s => boolR s).
+- refine (fun r β s0 s1 => _). exact (s0 r !).
+- refine (fun r β s0 s1 => _). exact (s0 r !).
+- refine (fun r β s0 s1 => _). exact (s1 r !).
+- refine (fun r β s0 s1 => _). exact (s1 r !).
 Defined.
 
 Definition bool1 {p} : @El1 p Type0 Type1 bool0.
@@ -472,7 +276,7 @@ Definition Arr0 {p}
   (B1 : @El1 p Type0 Type1 B0) :
   @El0 p Type0.
 Proof.
-unshelve refine (fun q α => mkYFT _ _ _ _).
+unshelve econstructor.
 - unshelve refine (fun r β =>
   forall
   (x0 : El0 (α ∘ β · A0))
@@ -487,17 +291,19 @@ unshelve refine (fun q α => mkYFT _ _ _ _).
   (B0 r (α ∘ β)).(yft1) r ! (fun r' β' => _)).
   unshelve refine (cast0 B0 B1 (α ∘ β) β' _).
   exact (f r' β' (β' · x0) (β' · x1)).
-- unshelve refine (fun r β b e l le l' => _).
-  unshelve econstructor.
-  + unfold yt_funct ; simpl.
-    unshelve econstructor ; simpl.
-    * refine (fun r0 β0 x0 x1 => _).
-      apply falso.
-    * refine (fun r0 β0 x0 x1 => _).
-      apply sfalso.
-  + refine (fun r0 β0 Hβ0 => _).
-    unfold ytEl_funct ; simpl.
-    apply sfalso.
+- refine (fun r β s0 s1 x0 x1 => _). apply falso.
+  (* simpl in s0 ; simpl in s1.
+  refine (J_seq _ _ (fun X _ => yft0 (X r (β ∘ side_1)) r !) _ _ (ssym (B1 q α))).
+  unshelve refine (yftfibl0 (B0 q α) r β _ _).
+  + refine (fun r0 β0 => _).
+    refine (J_seq _ _ (fun X _ => yft0 (X r0 (β ∘ side_0 ∘ β0)) r0 !) _ _ (B1 q α)).
+    unshelve refine (s0 r0 β0 _ _).
+    *
+    *
+  +  *)
+- refine (fun r β s0 s1 x0 x1 => _). apply falso.
+- refine (fun r β s0 s1 x0 x1 => _). apply sfalso.
+- refine (fun r β s0 s1 x0 x1 => _). apply sfalso.  
 Defined.
 
 Definition Arr1 {p}
@@ -590,8 +396,10 @@ unshelve econstructor.
   exact (SigmaT (α ∘ β ⋅ A0) (α ∘ β ⋅ A1) (α ∘ β ⋅ P0) (α ∘ β ⋅ P1)).
 - refine (fun r β => _).
   exact (SigmaR (α ∘ β ⋅ A0) (α ∘ β ⋅ A1) (α ∘ β ⋅ P0) (α ∘ β ⋅ P1)).
-- refine (fun r β b e l le l' => _).
-  apply falso.
+- refine (fun r β s0 s1 => _). apply falso.
+- refine (fun r β s0 s1 => _). apply falso.
+- refine (fun r β s0 s1 => _). apply sfalso.
+- refine (fun r β s0 s1 => _). apply sfalso.
 Defined.
 
 Definition Sigma1 {p}
@@ -705,7 +513,6 @@ Admitted.
 | Sigma_c : forall (a0 : El0 A0) (a1 : El1 A0 A1 a0)
   (b0 : El0 (app0 P0 a0 a1)) (b1 : El1 _ (app1 P1 a0 a1) b0),
   SigmaT A0 A1 P0 P1.
-
 Definition SigmaT_funct {p}
   {A0 : @El0 p Type0}
   {A1 : @El1 p Type0 Type1 A0}
@@ -717,7 +524,6 @@ Proof.
 intros [a0 a1 b0 b1].
 exact (Sigma_c _ _ _ _ (α ⋅ a0) (α ⋅ a1) (α ⋅ b0) (α ⋅ b1)).
 Defined.
-
 Definition fst0_SigmaT {p}
   {A0 : @El0 p Type0}
   {A1 : @El1 p Type0 Type1 A0}
@@ -729,7 +535,6 @@ Proof.
 destruct x0 as [a0 a1 b0 b1].
 exact a0.
 Defined.
-
 Definition fst1_SigmaT {p}
   {A0 : @El0 p Type0}
   {A1 : @El1 p Type0 Type1 A0}
@@ -741,7 +546,6 @@ Proof.
 destruct x0 as [a0 a1 b0 b1].
 exact a1.
 Defined.
-
 Definition snd_SigmaT {p}
   {A0 : @El0 p Type0}
   {A1 : @El1 p Type0 Type1 A0}
@@ -754,7 +558,6 @@ unfold fst0_SigmaT. unfold fst1_SigmaT.
 destruct x0 as [a0 a1 b0 b1].
 exact b0.
 Defined.
-
 Definition seq_SigmaT_transp {p}
   {A0 : @El0 p Type0}
   {A1 : @El1 p Type0 Type1 A0}
@@ -772,7 +575,6 @@ refine (J_seq _ (fst0_SigmaT a0)
     (J_seqs _ (fst0_SigmaT a0) (fun y _ => El1 A0 A1 y) (fst1_SigmaT a0) x e)))
   x (fst0_SigmaT b0) H).
 Defined.
-
 Definition seq_SigmaT {p}
   {A0 : @El0 p Type0}
   {A1 : @El1 p Type0 Type1 A0}
@@ -797,7 +599,6 @@ simpl in H1.
 destruct H1.
 reflexivity.
 Defined.
-
 Definition SigmaR {p}
   (A0 : @El0 p Type0)
   (A1 : @El1 p Type0 Type1 A0)
@@ -805,7 +606,6 @@ Definition SigmaR {p}
   (P1 : El1 _ (Arr1 A0 A1 Type0 Type1) P0)
   : (forall q (α : q ≤ p), SigmaT (α ⋅ A0) (α ⋅ A1) (α ⋅ P0) (α ⋅ P1)) -> SProp :=
 fun s => s ≡ fun q α => SigmaT_funct α (s p !).
-
 Definition Sigma0 {p}
   (A0 : @El0 p Type0)
   (A1 : @El1 p Type0 Type1 A0)
@@ -822,7 +622,6 @@ unshelve econstructor.
 - refine (fun r β b e l le l' => _).
   apply falso.
 Defined.
-
 Definition Sigma1 {p}
   (A0 : @El0 p Type0)
   (A1 : @El1 p Type0 Type1 A0)
@@ -873,14 +672,14 @@ Definition Prod0 {p}
   (B1 : El1 (Arr0 A0 A1 Type0 Type1) (Arr1 A0 A1 Type0 Type1) B0)
   : @El0 p Type0.
 Proof.
-unshelve refine (fun q α => mkYFT _ _ _ _).
-+ unshelve refine (fun r β =>
+unshelve econstructor.
+- unshelve refine (fun r β =>
   forall
   (x0 : El0 (α ∘ β · A0))
   (x1 : El1 (α ∘ β · A0) (α ∘ β · A1) x0)
   ,
   (B0 r (α ∘ β) x0 x1).(yft0) r !).
-+ unshelve refine (fun r β f0 =>
+- unshelve refine (fun r β f0 =>
   forall
   (x0 : El0 (α ∘ β · A0))
   (x1 : El1 (α ∘ β · A0) (α ∘ β · A1) x0)
@@ -890,8 +689,10 @@ unshelve refine (fun q α => mkYFT _ _ _ _).
     (fun r3 (β3 : r3 ≤ r) => B0 r3 (α ∘ β ∘ β3) (β3 · x0) (β3 · x1))
     (fun r3 (β3 : r3 ≤ r) => B1 r3 (α ∘ β ∘ β3) (β3 · x0) (β3 · x1))
     _ ! _ β2 (f0 r2 _ (β2 · x0) (β2 · x1))).
-+ refine (fun q α => _).
-  apply falso.
+- refine (fun r β s0 s1 => _). apply falso.
+- refine (fun r β s0 s1 => _). apply falso.
+- refine (fun r β s0 s1 => _). apply sfalso.
+- refine (fun r β s0 s1 => _). apply sfalso.
 Defined.
 
 Definition Prod1 {p}
@@ -1003,13 +804,15 @@ Definition eq0 {p}
   (y1 : El1 A0 A1 y0) :
   @El0 p Type0.
 Proof.
-unshelve refine (fun q α => mkYFT _ _ _ _).
+unshelve econstructor.
 - unshelve refine (fun r β => _).
   exact (cube_eq ((α ∘ β) · A0) ((α ∘ β) · A1) ((α ∘ β) · x0) ((α ∘ β) · y0)).
 - unshelve refine (fun r β s => _). simpl in s.
   exact (cube_eqR ((α ∘ β) · A0) ((α ∘ β) · A1) ((α ∘ β) · x0) ((α ∘ β) · y0) s).
-- unshelve refine (fun r β b e l le l' => _).
-  apply falso. (** TODO **)
+- refine (fun r β s0 s1 => _). apply falso.
+- refine (fun r β s0 s1 => _). apply falso.
+- refine (fun r β s0 s1 => _). apply sfalso.
+- refine (fun r β s0 s1 => _). apply sfalso.
 Defined.
 
 Definition eq1 {p}
@@ -1049,4 +852,122 @@ Proof.
 unshelve refine (fun q α => _).
 reflexivity.
 Defined.
+(* 
+(* shifted types *)
 
+Record shifted_ty {p} : Type :=
+mkST {
+  st_t0 : @El0 (S p) Type0 ;
+  st_t1 : @El1 (S p) Type0 Type1 st_t0 ;
+}.
+
+Definition st_funct {p} {q} (α : q ≤ p) :
+  @shifted_ty p -> @shifted_ty q.
+Proof.
+unshelve refine (fun x => _).
+unshelve econstructor.
+- exact (promote α ⋅ x.(st_t0)).
+- exact (promote α ⋅ x.(st_t1)).
+Defined.
+
+Definition shifted_tyR {p} :
+ (forall q (α : q ≤ p), @shifted_ty q) -> SProp :=
+fun s => s ≡ fun q α => st_funct α (s p !).
+
+Definition shiftedType0 {p}
+  : @El0 p Type0.
+Proof.
+refine (fun q α => _).
+unshelve econstructor. 
+- refine (fun r β => _).
+  exact (@shifted_ty r).
+- refine (fun r β s => _). simpl in s.
+  exact (shifted_tyR s).
+- refine (fun r β s0 s1 => _). apply falso.
+- refine (fun r β s0 s1 => _). apply falso.
+- refine (fun r β s0 s1 => _). apply sfalso.
+- refine (fun r β s0 s1 => _). apply sfalso.  
+Defined.
+
+Definition shiftedType1 {p}
+  : @El1 p Type0 Type1 shiftedType0.
+Proof.
+refine (fun q α => _). reflexivity.
+Defined.
+
+Definition shiftedTypeStart0 {p}
+  (A0 : @El0 p shiftedType0)
+  (A1 : @El1 p shiftedType0 shiftedType1 A0) :
+  @El0 p Type0.
+Proof.
+refine (fun q α => _).
+refine ((side_0 ⋅ st_t0 (A0 q α)) q !). 
+Defined.
+
+Definition shiftedTypeStart1 {p}
+  (A0 : @El0 p shiftedType0)
+  (A1 : @El1 p shiftedType0 shiftedType1 A0) :
+  @El1 p Type0 Type1 (shiftedTypeStart0 A0 A1).
+Proof.
+refine (fun q α => _). 
+refine (J_seqs _ _ (fun X _ => yftR (fun r β => st_t0 (X r β) r side_0 )) _ (α ⋅ A0) (ssym (A1 q α))).
+refine ((side_0 ⋅ st_t1 (A0 q α)) q !).
+Defined.
+
+Definition shiftedTypeEnd0 {p}
+  (A0 : @El0 p shiftedType0)
+  (A1 : @El1 p shiftedType0 shiftedType1 A0) :
+  @El0 p Type0.
+Proof.
+refine (fun q α => _).
+refine ((side_1 ⋅ st_t0 (A0 q α)) q !). 
+Defined.
+
+Definition shiftedTypeEnd1 {p}
+  (A0 : @El0 p shiftedType0)
+  (A1 : @El1 p shiftedType0 shiftedType1 A0) :
+  @El1 p Type0 Type1 (shiftedTypeEnd0 A0 A1).
+Proof.
+refine (fun q α => _). 
+refine (J_seqs _ _ (fun X _ => yftR (fun r β => st_t0 (X r β) r side_1)) _ (α ⋅ A0) (ssym (A1 q α))).
+refine ((side_1 ⋅ st_t1 (A0 q α)) q !).
+Defined.
+
+(* transport boils down to a statement about shifted types *)
+
+Definition transp0 {p}
+  (A0 : @El0 p shiftedType0)
+  (A1 : @El1 p shiftedType0 shiftedType1 A0)
+  (s0 : El0 (shiftedTypeStart0 A0 A1))
+  (s1 : El1 _ (shiftedTypeStart1 A0 A1) s0)
+  : El0 (shiftedTypeEnd0 A0 A1).
+Proof.
+refine (fun q α => _).
+unfold shiftedTypeEnd0 ; simpl.
+refine (J_seq _ _ (fun X _ => yft0 (X q side_1) q !) _ _ (ssym (st_t1 (A0 q α) (S q) !))).
+change (yft0 (st_t0 (A0 q α) (S q) !) q side_1).
+
+pose proof (yftfibl0 (st_t0 (A0 q α) (S q) !) q !) as fib0.
+unshelve refine (fib0 _ _).
+- refine (fun r β => _).
+  refine (J_seq _ _ (fun X _ => yft0 (X r (side_0 ∘ β)) r !) _ _ (st_t1 (A0 q α) (S q) !)).
+  refine (J_seq _ _ (fun X _ => yft0 (st_t0 (X r β) r side_0) r !) _ _ (A1 q α)).
+  refine (s0 r (α ∘ β)).
+- refine (fun r β => _).
+  apply sfalso.
+Defined.
+
+Definition transp1 {p}
+  (A0 : @El0 p shiftedType0)
+  (A1 : @El1 p shiftedType0 shiftedType1 A0)
+  (s0 : El0 (shiftedTypeStart0 A0 A1))
+  (s1 : El1 _ (shiftedTypeStart1 A0 A1) s0)
+  : El1 _ (shiftedTypeEnd1 A0 A1) (transp0 A0 A1 s0 s1).
+Proof.
+refine (fun q α => _).
+unfold shiftedTypeEnd0 ; simpl.
+unfold transp0 ; simpl.
+unfold cast0 ; simpl.
+Admitted.
+
+ *)
